Main.v
@@ -18,21 +18,11 @@ Module Make (Export D : Defs.T).
   | Rej : string -> parse_result
   | Err : parse_error -> parse_result.
 
+  (* to do : this can be replaced by parse *)
   Definition parseSymbol (g : grammar)
-             (s : symbol)
-             (w : list token) : parse_result :=
-    match parse g [s] w with
-    | Accept [v] => Acc v
-    | Ambig  [v] => Amb v
-    | Reject str => Rej str
-    | Error e    => Err e
-    | _          => Err InvalidState
-    end.
-
-  Definition parseSymbol_opt (g : grammar)
-                             (s : symbol)
-                             (w : list token) : parse_result :=
-    match parse_opt g [s] w with
+                         (x : nonterminal)
+                         (w : list token) : parse_result :=
+    match parse g x w with
     | Accept [v] => Acc v
     | Ambig  [v] => Amb v
     | Reject str => Rej str
@@ -44,26 +34,26 @@ Module Make (Export D : Defs.T).
 
   Theorem parseSymbol_sound_unambig :
     forall (g : grammar)
-           (s : symbol)
+           (x : nonterminal)
            (w : list token)
            (t : tree),
       no_left_recursion g
-      -> parseSymbol g s w = Acc t
-      -> sym_derivation g s w t
-         /\ (forall t', sym_derivation g s w t' -> t' = t).
+      -> parseSymbol g x w = Acc t
+      -> sym_derivation g (NT x) w t
+         /\ (forall t', sym_derivation g (NT x) w t' -> t' = t).
   Proof.
-    intros g s w t hn hp.
+    intros g x w t hn hp.
     unfold parseSymbol in hp.
     destruct (parse _ _ _) as [v | v | str | e] eqn:hp'; tc.
     - apply parse_sound_unambig in hp'; auto.
       destruct hp' as (hg & ha).
       (* lemma *)
       inv hg.
-      inv H4; rewrite app_nil_r in *.
+      inv H4; rew_anr.
       inv hp.
       split; auto.
       intros g' hs.
-      assert (gamma_derivation g [s] wpre [g']).
+      assert (gamma_derivation g [NT x] wpre [g']).
       { rew_nil_r wpre; eauto. }
       apply ha in H; inv H; auto.
     - destruct v as [ | ? [ | ? ? ]]; tc.
@@ -71,15 +61,15 @@ Module Make (Export D : Defs.T).
 
   Theorem parseSymbol_sound_ambig :
     forall (g : grammar)
-           (s : symbol)
+           (x : nonterminal)
            (w : list token)
            (t : tree),
       no_left_recursion g
-      -> parseSymbol g s w = Amb t
-      -> sym_derivation g s w t
-         /\ (exists t', sym_derivation g s w t' /\ t' <> t).
+      -> parseSymbol g x w = Amb t
+      -> sym_derivation g (NT x) w t
+         /\ (exists t', sym_derivation g (NT x) w t' /\ t' <> t).
   Proof.
-    intros g s w t hn hp.
+    intros g x w t hn hp.
     unfold parseSymbol in hp.
     destruct (parse _ _ _) as [v | v | str | e] eqn:hp'; tc.
     - destruct v as [ | ? [ | ? ? ]]; tc.
@@ -100,13 +90,13 @@ Module Make (Export D : Defs.T).
 
   Theorem parseSymbol_error_free :
     forall (g  : grammar)
-           (s  : symbol)
+           (x  : nonterminal)
            (ts : list token)
            (e  : parse_error),
       no_left_recursion g
-      -> parseSymbol g s ts <> Err e.
+      -> parseSymbol g x ts <> Err e.
   Proof.
-    intros g s ts e hn; unfold not; intros hp.
+    intros g x ts e hn; unfold not; intros hp.
     unfold parseSymbol in hp.
     destruct (parse _ _ _) eqn:hp'; tc.
     - apply parse_sound_unambig in hp'; auto.
@@ -115,23 +105,23 @@ Module Make (Export D : Defs.T).
     - apply parse_sound_ambig in hp'; auto.
       destruct hp' as (hg & _).
       inv hg. inv H4. tc.
-    - apply parser_terminates_without_error in hp'; auto.
+    - apply parse_terminates_without_error in hp'; auto.
   Qed.
 
   (* Completeness theorems for unambiguous and ambiguous derivations *)
 
   Theorem parseSymbol_complete_unique_derivation :
     forall (g : grammar)
-           (s : symbol)
+           (x : nonterminal)
            (w : list token)
            (t : tree),
       no_left_recursion g
-      -> sym_derivation g s w t
-      -> (forall t', sym_derivation g s w t' -> t' = t)
-      -> parseSymbol g s w = Acc t.
+      -> sym_derivation g (NT x) w t
+      -> (forall t', sym_derivation g (NT x) w t' -> t' = t)
+      -> parseSymbol g x w = Acc t.
   Proof.
-    intros g s w t hn hs ha.
-    assert (hg : gamma_derivation g [s] w [t]).
+    intros g x w t hn hs ha.
+    assert (hg : gamma_derivation g [NT x] w [t]).
     { rew_nil_r w; eauto. }
     apply parse_complete_unique_derivation in hg; auto.
     - unfold parseSymbol; rewrite hg; auto.
@@ -146,29 +136,29 @@ Module Make (Export D : Defs.T).
 
   Theorem parseSymbol_complete_ambiguous_derivations :
     forall (g    : grammar)
-           (s    : symbol)
+           (x    : nonterminal)
            (w    : list token)
            (t t' : tree),
       no_left_recursion g
-      -> sym_derivation g s w t
-      -> sym_derivation g s w t'
+      -> sym_derivation g (NT x) w t
+      -> sym_derivation g (NT x) w t'
       -> t <> t'
-      -> exists t'', parseSymbol g s w = Amb t''.
+      -> exists t'', parseSymbol g x w = Amb t''.
   Proof.
-    intros g s w t t' hn hs hs' hneq.
-    assert (hg : gamma_derivation g [s] w [t]).
+    intros g x w t t' hn hs hs' hneq.
+    assert (hg : gamma_derivation g [NT x] w [t]).
     { rew_nil_r w; eauto. }
-    assert (hg' : gamma_derivation g [s] w [t']).
+    assert (hg' : gamma_derivation g [NT x] w [t']).
     { rew_nil_r w; eauto. }
     assert (hneq' : [t] <> [t']).
     { unfold not; intros ?; subst; tc. }
     eapply parse_complete_ambiguous_derivations in hg; eauto.
-    destruct hg as (v'' & hp).
+    destruct hg as (v'' & hp & hg).
     pose proof hp as hp'.
     apply parse_sound_ambig in hp; auto.
-    destruct hp as (hg & _).
-    inv hg.
-    inv H4; rewrite app_nil_r in *.
+    destruct hp as (hg'' & _).
+    inv hg''.
+    inv H4; rew_anr.
     unfold parseSymbol.
     rewrite hp'; eauto.
   Qed.
